mc_reify/bool_funcs.v
@@ -1,0 +1,73 @@
+Require Import veric.expr.
+Require Import veric.SeparationLogic.
+
+Definition denote_tc_assert_b_norho a:=
+match a with 
+| tc_TT => true
+| _ => false
+end.
+
+Definition tc_expr_b_norho Delta e :=
+denote_tc_assert_b_norho (typecheck_expr Delta e).
+
+Definition tc_temp_id_b_norho id t Delta e:=
+denote_tc_assert_b_norho (typecheck_temp_id id t Delta e).
+
+Lemma tc_expr_b_sound : 
+forall e Delta rho,
+tc_expr_b_norho Delta e = true ->
+tc_expr Delta e rho .
+Proof.
+intros.
+unfold tc_expr, tc_expr_b_norho in *. 
+destruct (typecheck_expr Delta e); simpl in *; unfold_lift; simpl; auto; try congruence. 
+Qed.
+
+Lemma tc_temp_id_b_sound : 
+forall id t Delta e rho,
+tc_temp_id_b_norho id t Delta e= true ->
+tc_temp_id id t Delta e rho .
+Proof.
+intros. 
+unfold tc_temp_id, tc_temp_id_b_norho in *.
+destruct (typecheck_temp_id id t Delta e); simpl in *; unfold_lift; simpl; auto; try congruence.
+Qed.
+
+Fixpoint msubst_eval_expr_norho (T1: PTree.t val) (T2: PTree.t (type * val)) (e: Clight.expr) : option val :=
+  match e with
+  | Econst_int i ty => Some (Vint i)
+  | Econst_long i ty => Some (Vlong i)
+  | Econst_float f ty => Some (Vfloat f)
+  | Econst_single f ty => Some (Vsingle f)
+  | Etempvar id ty => PTree.get id T1
+  | Eaddrof a ty => msubst_eval_lvalue_norho T1 T2 a 
+  | Eunop op a ty =>  option_map (eval_unop op (typeof a)) (msubst_eval_expr_norho T1 T2 a) 
+  | Ebinop op a1 a2 ty => match (msubst_eval_expr_norho T1 T2 a1), (msubst_eval_expr_norho T1 T2 a2) with
+                            | Some v1, Some v2 => Some (eval_binop op (typeof a1) (typeof a2) v1 v2) 
+                            | _, _ => None
+                          end
+  | Ecast a ty => option_map (eval_cast (typeof a) ty) (msubst_eval_expr_norho T1 T2 a)
+  | Evar id ty => option_map (deref_noload ty)
+                    match PTree.get id T2 with
+                    | Some (ty', v) =>
+                      if eqb_type ty ty'
+                      then Some v
+                      else None
+                    | None => None
+                    end
+  | Ederef a ty => option_map (deref_noload ty) (option_map force_ptr (msubst_eval_expr_norho T1 T2 a))
+  | Efield a i ty => option_map (deref_noload ty) (option_map (eval_field (typeof a) i) (msubst_eval_lvalue_norho T1 T2 a))
+  end
+  with msubst_eval_lvalue_norho (T1: PTree.t val) (T2: PTree.t (type * val)) (e: Clight.expr) : option val := 
+  match e with 
+  | Evar id ty => match PTree.get id T2 with
+                  | Some (ty', v) =>
+                    if eqb_type ty ty'
+                    then Some v
+                    else None
+                  | None => None
+                  end
+  | Ederef a ty => option_map force_ptr (msubst_eval_expr_norho T1 T2 a)
+  | Efield a i ty => option_map (eval_field (typeof a) i) (msubst_eval_lvalue_norho T1 T2 a)
+  | _  => Some Vundef
+  end.
