mc_reify/local2list.v
@@ -1,0 +1,145 @@
+Require Import floyd.base.
+Require Import floyd.client_lemmas.
+Require Import floyd.assert_lemmas.
+Require Import floyd.closed_lemmas.
+Require Import floyd.canonicalize.
+Require Import floyd.forward_lemmas.
+Require Import floyd.call_lemmas.
+Require Import floyd.extcall_lemmas.
+Require Import floyd.type_id_env.
+
+Local Open Scope logic.
+
+Inductive local2list:
+  list (environ -> Prop) -> list (ident * val) -> list (ident * (type * val)) -> list (environ -> Prop) -> Prop :=
+  | local2list_nil:
+      local2list nil (nil) (nil) nil
+  | local2list_temp_var: forall v i Q T1 T2 Q',
+      local2list Q T1 T2 Q'->
+      local2list (`(eq v) (eval_id i) :: Q) (cons (i, v) T1) T2 Q'
+  | local2list_gl_var: forall v i t Q T1 T2 Q',
+      local2list Q T1 T2 Q'->
+      local2list (`(eq v) (eval_var i t) :: Q) T1 (cons (i, (t, v)) T2) Q'
+  | local2list_unknown: forall Q0 Q T1 T2 Q',
+      local2list Q T1 T2 Q'->
+      local2list (Q0 :: Q) T1 T2 (Q0 :: Q').
+(* repeat constructor will try the first succesful tactic. So local2list_temp_ *)
+(* var, local2list_gl_var will be used whenever is possible before local2list_*)
+(* unknown.                                                                     *)
+
+Module TEST.
+Goal False.
+evar (T1: list (ident * val)).
+evar (T2: list (ident * (type * val))).
+evar (Q' : list (environ -> Prop)).
+
+assert (local2list  ((`(eq Vundef) (eval_id 1%positive)) :: (`(eq (Vint (Int.repr 1))) (eval_id 1%positive)) :: 
+   (`(eq 1 3)) :: nil)
+  T1 T2 Q').
+subst T1 T2 Q'.
+repeat constructor; repeat simpl; auto.
+simpl in H.
+Abort.
+
+Goal False.
+evar (T1: list (ident * val)).
+evar (T2: list (ident * (type * val))).
+evar (Q' : list (environ -> Prop)).
+assert (local2list ((`(eq Vundef) (eval_id 1%positive))::nil) T1 T2 Q').
+subst T1 T2 Q'.
+repeat constructor; repeat simpl; auto.
+Abort.
+End TEST.
+
+Definition localtempD (p : (ident * val)) := let (i, v) := p in `(eq v) (eval_id i).
+Definition localvarD (p : ident * (type * val))  := let (i, tv) := p in `(eq (snd tv)) (eval_var i (fst tv)).
+
+Definition LocallistD (T1: list (ident * val)) (T2: list (ident * (type * val))) (Q: list (environ -> Prop)) :=
+  map localtempD T1 ++ map localvarD T2 ++ Q.
+
+Lemma PTree_elements_set: forall {A} i (v: A) elm T,
+  In elm (PTree.elements (PTree.set i v T)) ->
+  elm = (i, v) \/ In elm (PTree.elements T).
+Proof.
+  intros.
+  destruct elm as [i' v'].
+  apply PTree.elements_complete in H.
+  destruct (ident_eq i i').
+  + subst.
+    rewrite PTree.gss in H.
+    inversion H.
+    subst.
+    left; auto.
+  + rewrite PTree.gso in H by auto.
+    right.
+    apply PTree.elements_correct.
+    auto.
+Qed.
+
+Lemma LOCALx_shuffle: forall P Q Q' R,
+  (forall Q0, In Q0 Q' -> In Q0 Q) ->
+  PROPx P (LOCALx Q (SEPx R)) |-- PROPx P (LOCALx Q' (SEPx R)).
+Proof.
+  intros.
+  induction Q'; [simpl; intro; normalize |].
+  pose proof (H a (or_introl _ eq_refl)).
+  rewrite <- insert_local.
+  apply andp_right.
+  + clear -H0.
+    induction Q; [inversion H0 |].
+    rewrite <- insert_local.
+    simpl in H0; inversion H0.
+    - subst.
+      apply andp_left1.
+      apply derives_refl.
+    - apply andp_left2.
+      apply IHQ, H.
+  + apply IHQ'.
+    intros.
+    apply H.
+    simpl.
+    right.
+    apply H1.
+Qed.
+
+
+Lemma local2list_soundness: forall P Q R T1 T2 Q',
+  local2list Q T1 T2 Q' ->
+  PROPx P (LOCALx Q (SEPx R)) = PROPx P (LOCALx (LocallistD T1 T2 Q') (SEPx R)).
+Proof.
+  intros.
+  apply pred_ext.
+* induction H.
+  + auto.
+  + eapply derives_trans.
+    - rewrite <- insert_local.
+      apply andp_derives; [apply derives_refl | exact IHlocal2list].
+    - rewrite insert_local. auto.
+  + eapply derives_trans.
+    - rewrite <- insert_local.
+      apply andp_derives; [apply derives_refl | exact IHlocal2list].
+    - rewrite insert_local.
+      apply LOCALx_shuffle.
+      intros. unfold LocallistD in *.
+      simpl.
+      repeat rewrite in_app in *. simpl in *. intuition. 
+  + eapply derives_trans.
+    - rewrite <- insert_local.
+      apply andp_derives; [apply derives_refl | exact IHlocal2list].
+    - rewrite insert_local.
+      apply LOCALx_shuffle. intros.
+      unfold LocallistD in *. repeat rewrite in_app in *. simpl in *.
+      intuition.
+*induction H.
+  + auto.
+  + rewrite <- insert_local. 
+Admitted.
+
+Fixpoint locallist2ptree {A : Type} (l : list (ident * A)) (p : PTree.t A) (e : list Prop) : ((PTree.t A) * (list Prop)) :=
+match l with
+| (id, v) :: t => match (p ! id) with
+                    | Some (v2) => locallist2ptree t p ((v = v2) :: e)
+                    | None => locallist2ptree t (PTree.set id v p) e
+                  end
+| nil => (p, e)
+end.
