mc_reify/set_reif.v
@@ -1,0 +1,249 @@
+Require Import floyd.proofauto. 
+Require Import funcs.
+Require Import bool_funcs.
+Require Import MirrorCore.Lambda.ExprCore.
+
+
+
+Definition appR (e1 : func') e2 := App (@Inj typ func (inr e1)) (e2). 
+Definition injR (e1 : func') := @Inj typ func (inr e1).
+
+Fixpoint msubst_eval_expr_reif (T1: PTree.t (ExprCore.expr typ func)) (T2: PTree.t (type * (ExprCore.expr typ func))) (e: Clight.expr) : option (ExprCore.expr typ func) :=
+  match e with
+  | Econst_int i ty => Some (appR (Value fVfloat) (injR (Const (fint i))))
+  | Econst_long i ty => Some (appR (Value fVlong) (injR (Const (fint64 i))))
+  | Econst_float f ty => Some (appR (Value fVfloat) (injR (Const (ffloat f))))
+  | Econst_single f ty => Some (appR (Value fVsingle) (injR (Const (ffloat32 f))))
+  | Etempvar id ty => PTree.get id T1
+  | Eaddrof a ty => msubst_eval_lvalue_reif T1 T2 a 
+  | Eunop op a ty =>  option_map (appR (Eval_f (feval_unop op (typeof a))))
+                                       (msubst_eval_expr_reif T1 T2 a) 
+  | Ebinop op a1 a2 ty => match (msubst_eval_expr_reif T1 T2 a1), (msubst_eval_expr_reif T1 T2 a2) with
+                            | Some v1, Some v2 => Some 
+                                (App (appR (Eval_f (feval_binop op 
+                                         (typeof a1) (typeof a2))) v1) v2) 
+                            | _, _ => None
+                          end
+  | Ecast a ty => option_map (appR (Eval_f (feval_cast (typeof a) ty))) (msubst_eval_expr_reif T1 T2 a)
+  | Evar id ty => option_map (appR (Eval_f (fderef_noload ty)))
+                    match PTree.get id T2 with
+                    | Some (ty', v) =>
+                      if eqb_type ty ty'
+                      then Some v
+                      else None
+                    | None => None
+                    end
+  | Ederef a ty => 
+      option_map (appR (Eval_f (fderef_noload ty))) 
+                 (option_map (appR (Other (fforce_ptr)))
+                             (msubst_eval_expr_reif T1 T2 a))
+  | Efield a i ty => option_map (appR (Eval_f (fderef_noload ty))) 
+                                (option_map (appR (Eval_f (feval_field (typeof a) i))) (msubst_eval_lvalue_reif T1 T2 a))
+  end
+  with msubst_eval_lvalue_reif (T1: PTree.t (ExprCore.expr typ func)) (T2: PTree.t (type * (ExprCore.expr typ func))) (e: Clight.expr) : option (ExprCore.expr typ func) := 
+  match e with 
+  | Evar id ty => match PTree.get id T2 with
+                  | Some (ty', v) =>
+                    if eqb_type ty ty'
+                    then Some v
+                    else None
+                  | None => None
+                  end
+  | Ederef a ty => option_map (appR (Other fforce_ptr)) (msubst_eval_expr_reif T1 T2 a)
+  | Efield a i ty => option_map (appR (Eval_f (feval_field (typeof a) i))) (msubst_eval_lvalue_reif T1 T2 a)
+  | _  => Some (injR (Value fVundef))
+  end.
+
+Lemma Forall_reverse :
+forall A P (l: list A),
+Forall P l <->
+Forall P (rev l). 
+Proof.
+intros.
+split; intros.
+ + rewrite Forall_forall in *.
+   intros. destruct l.
+      - apply H. auto.
+      - simpl in *. apply in_app in H0.
+        destruct H0. apply H; auto.
+        right. apply in_rev; auto.
+        apply H.  left. simpl in H0. intuition.
+ + rewrite Forall_forall in *; intros.
+   destruct l.
+   inversion H0.
+   destruct H0.
+   subst.
+   simpl in *. apply H. apply in_app. right. constructor. auto.
+   apply H. simpl. apply in_app. left. apply in_rev in H0. auto.
+Qed.
+
+Lemma in_fst :
+forall T T2 (p : T) (v: T2) l, 
+In (p, v) l -> In p (map fst l).
+Proof.
+intros.
+  + induction l. auto.
+      - simpl in *. intuition.
+        destruct a. left. simpl. congruence.
+Qed.
+
+
+Lemma elt_eq : forall T l p (v:T) v0 ls, 
+(p, v0) :: l = rev (PTree.elements (PTree.set p v ls)) ->
+v = v0.
+Proof.
+intros.
+assert (In (p, v) (rev (PTree.elements (PTree.set p v ls)))).
+  { rewrite <- in_rev. apply PTree.elements_correct. rewrite PTree.gss. auto. }
+assert (X := PTree.elements_keys_norepet (PTree.set p v ls)).
+assert (In (p, v0) (rev (PTree.elements (PTree.set p v ls)))).
+  { rewrite <- list_norepet_rev in X. rewrite <- map_rev in X. unfold PTree.elt in *. 
+    rewrite <- H in *. simpl in *. intuition. }
+rewrite <- in_rev in H1. 
+  rewrite <- list_norepet_rev in X. rewrite <- map_rev in X. unfold PTree.elt in *.
+  rewrite in_rev in H1.  
+    rewrite <- H in *. simpl in *. clear - X H0 H1. intuition; try congruence.
+    inversion X; subst. intuition. apply in_fst in H. intuition.
+    inversion X. subst. intuition. apply in_fst in H. intuition.
+Qed.
+
+Definition tempD' := (fun Q i v => `(eq v) (eval_id i) :: Q).
+Definition localD' := (fun Q i tv => `(eq (snd tv)) (eval_var i (fst tv)) :: Q).
+Definition LocalD_app (T1: PTree.t val) (T2: PTree.t (type * val)) (Q: list (environ -> Prop)) :=
+  (PTree.fold tempD' T1 nil) ++ 
+ (PTree.fold localD' T2 nil) ++ Q.
+
+
+Lemma localD_app_eq : forall t2 q, PTree.fold localD' t2 q = PTree.fold localD' t2 nil ++ q.
+Proof.
+intros.
+repeat rewrite PTree.fold_spec.
+simpl in *. repeat rewrite <- fold_left_rev_right.
+induction (rev (PTree.elements t2)).
+  + reflexivity.
+  + simpl. rewrite IHl. auto.
+Qed.
+
+Lemma tempD_app_eq : forall t2 q, PTree.fold tempD' t2 q = PTree.fold tempD' t2 nil ++ q.
+intros.
+repeat rewrite PTree.fold_spec.
+simpl in *. repeat rewrite <- fold_left_rev_right.
+induction (rev (PTree.elements t2)).
+  + reflexivity.
+  + simpl. rewrite IHl. auto.
+Qed.
+
+Lemma LocalD_app_eq : 
+forall t1 t2 q,
+LocalD t1 t2 q = LocalD_app t1 t2 q.
+Proof.
+intros.
+unfold LocalD, LocalD_app.
+simpl in *.
+rewrite localD_app_eq.
+rewrite tempD_app_eq. auto.
+Qed.
+
+Lemma fold_right_conj : 
+forall a b rho, 
+(fold_right (fun (x0 x1 : environ -> Prop) (x2 : environ) => x0 x2 /\ x1 x2) 
+     (`True) (a ++ b) rho) <-> ((fold_right (fun (x0 x1 : environ -> Prop) (x2 : environ) => x0 x2 /\ x1 x2) 
+     (`True) a rho /\ fold_right (fun (x0 x1 : environ -> Prop) (x2 : environ) => x0 x2 /\ x1 x2) 
+     (`True) b rho)).
+Proof.
+intros. 
+split; intros; induction a; simpl in *; intuition.
+Qed.
+
+
+Lemma semax_set_localD id e v ls vs:
+forall Espec Delta R ,
+tc_expr_b_norho Delta e= true ->
+tc_temp_id_b_norho id (typeof e) Delta e = true ->
+msubst_eval_expr_norho ls vs e = Some v ->
+@semax Espec Delta (assertD nil (localD ls vs) R)
+      (Sset id e)
+(normal_ret_assert (assertD nil (localD (PTree.set id v ls) vs) R)).
+Proof.
+(*intros.
+eapply semax_pre_simple; [ | apply forward_setx_closed_now].
+unfold assertD. apply andp_left2. apply derives_refl.
+Focus 2.
+rewrite Forall_forall. intros.
+induction R. inversion H2.
+simpl in H2. destruct H2. subst. auto with closed.
+intuition.
+apply andp_right. 
+apply andp_right; auto.
+intro rho.
+apply tc_expr_b_sound with (rho := rho) in H .
+unfold local. super_unfold_lift. apply prop_right. auto.
+unfold local. intro rho. super_unfold_lift.
+apply tc_temp_id_b_sound with (rho := rho) in H0. apply prop_right.
+auto.
+apply andp_left2. apply derives_refl.
+intros. go_lowerx. unfold normal_ret_assert.
+normalize. unfold assertD.
+autorewrite with subst.
+normalize. apply andp_right. apply prop_right. 
+Locate forward_setx_closed_now.
+eapply derives_trans with (SeparationLogic.subst id `v (assertD [] (localD ls vs) R) rho).
+
+rewrite LocalD_app_eq. 
+unfold LocalD_app. repeat rewrite fold_right_conj. 
+repeat split. 
+repeat rewrite PTree.fold_spec.
+repeat rewrite <-  fold_left_rev_right. 
+remember (rev (PTree.elements (PTree.set id v ls))).
+generalize dependent ls. generalize dependent id. generalize dependent v.
+induction l; intros.
+  + simpl. auto.
+  + simpl. split.
+     - destruct a. simpl in *.
+
+
+ 
+Check fold_right_app.
+rewrite <- fold_right_app.
+repeat rewrite fold_right_app.
+generalize dependent vs. generalize dependent ls.
+induction l0.
+  + simpl. induction l; intros.
+      - exact I.
+      - simpl. split. autorewrite with subst in *. destruct a. simpl. unfold_lift.
+        destruct (ident_eq p id). subst id.
+        assert (v=v0).
+          { apply elt_eq in Heql. subst. reflexivity. } 
+        subst. specialize (IHl ls). 
+
+apply PTree_elements_set in H1. destruct H1.
+congruence.
+rewrite <- list_norepet_rev in X. rewrite <- map_rev in X. unfold PTree.elt in *. 
+    rewrite <- H in *. simpl in *. 
+    inversion X; subst. 
+        
+ SearchAbout msubst_eval_expr.
+unfold_lift; reflexivity.
+unfold_lift; unfold_lift in H4. destruct H4; auto.
+remember (PTree.elements ls). induction l.
+unfold LocalD. repeat rewrite PTree.fold_spec.
+eapply forward_setx_closed_now; auto 50 with closed.
+ repeat rewrite <- Heql. simpl.
+rewrite <- fold_left_rev_right. 
+induction (rev (PTree.elements vs)). simpl. auto.
+simpl. rewrite Forall_forall. intros. simpl in H2.
+destruct H2. subst. auto with closed.
+rewrite Forall_forall in IHl. apply IHl. auto.
+admit. (*NOT TRUE. Lifts must be over all of R *)
+
+ SearchAbout Forall.
+
+ rewrite Forall_forall. intros.
+rewrite Forall_forall in IHl. apply IHl.
+
+
+Check PTree.elements_
+apply PTree.elements_compete in Heql.
+unfold LocalD. simpl.
+*)
+Admitted.
